zoo_eio/rcfd: Generalize to arbitrary fractional predicate.

theories/zoo_eio/rcfd.v
@@ -33,7 +33,6 @@ Implicit Types o : option val.
 
 Record metadata := {
   metadata_fd : val ;
-  metadata_chars : list ascii ;
   metadata_open : block_id ;
   metadata_tokens : gname ;
   metadata_lstate : gname ;
@@ -106,6 +105,8 @@ Qed.
 Section rcfd_G.
   Context `{rcfd_G : RcfdG Σ}.
 
+  Implicit Types Ψ : frac → iProp Σ.
+
   #[local] Definition tokens_auth' γ_tokens qs :=
     auth_gmultiset_auth γ_tokens (DfracOwn 1) qs.
   #[local] Definition tokens_auth γ qs :=
@@ -120,12 +121,12 @@ Section rcfd_G.
   #[local] Definition lstate_lb γ lstate :=
     auth_mono_lb _ γ.(metadata_lstate) lstate.
 
-  #[local] Definition inv_inner_open γ state ops : iProp Σ :=
+  #[local] Definition inv_inner_open γ Ψ state ops : iProp Σ :=
     ∃ q qs,
     ⌜ops = size qs ∧ set_fold Qp.add q qs = 1%Qp⌝ ∗
     ⌜state = Open⌝ ∗
     tokens_auth γ qs ∗
-    unix_fd_model γ.(metadata_fd) (DfracOwn q) γ.(metadata_chars).
+    Ψ q.
   #[local] Instance : CustomIpatFormat "inv_inner_open" :=
     "(
       %q{} &
@@ -133,15 +134,15 @@ Section rcfd_G.
       (-> & %Hqs{}) &
       {%H{eq};->} &
       Htokens_auth &
-      Hmodel_
+      HΨ{_{!}}
     )".
-  #[local] Definition inv_inner_closing_users γ state ops : iProp Σ :=
+  #[local] Definition inv_inner_closing_users γ Ψ state ops : iProp Σ :=
     ∃ q qs fn,
     ⌜ops = size qs ∧ 0 < size qs ∧ set_fold Qp.add q qs = 1%Qp⌝ ∗
     ⌜state = Closing fn⌝ ∗
     tokens_auth γ qs ∗
-    unix_fd_model γ.(metadata_fd) (DfracOwn q) γ.(metadata_chars) ∗
-    (unix_fd_model γ.(metadata_fd) (DfracOwn 1) γ.(metadata_chars) -∗ WP fn () {{ itype_unit }}).
+    Ψ q ∗
+    (Ψ 1%Qp -∗ WP fn () {{ itype_unit }}).
   #[local] Instance : CustomIpatFormat "inv_inner_closing_users" :=
     "(
       %q{} &
@@ -150,7 +151,7 @@ Section rcfd_G.
       ({%H{eq_ops};->} & %Hqs{}_size & %Hqs{}) &
       {%H{eq};->} &
       Htokens_auth &
-      Hmodel_ &
+      HΨ{_{!}} &
       Hfn{}
     )".
   #[local] Definition inv_inner_closing_no_users state : iProp Σ :=
@@ -163,16 +164,16 @@ Section rcfd_G.
       {%H{eq};->} &
       Hfn{}
     )".
-  #[local] Definition inv_inner l γ : iProp Σ :=
+  #[local] Definition inv_inner l γ Ψ : iProp Σ :=
     ∃ state lstate ops,
     l.[ops] ↦ #ops ∗
     l.[state] ↦ state_to_val γ state ∗
     lstate_auth γ lstate ∗
     match lstate with
     | LOpen =>
-        inv_inner_open γ state ops
+        inv_inner_open γ Ψ state ops
     | LClosingUsers =>
-        inv_inner_closing_users γ state ops
+        inv_inner_closing_users γ Ψ state ops
     | LClosingNoUsers =>
         inv_inner_closing_no_users state
     end.
@@ -186,18 +187,18 @@ Section rcfd_G.
       Hlstate_auth &
       Hlstate
     )".
-  Definition rcfd_inv t fd chars : iProp Σ :=
+  #[local] Definition inv' l γ Ψ :=
+    inv nroot (inv_inner l γ Ψ).
+  Definition rcfd_inv t fd Ψ : iProp Σ :=
     ∃ l γ,
     ⌜t = #l⌝ ∗
     ⌜fd = γ.(metadata_fd)⌝ ∗
-    ⌜chars = γ.(metadata_chars)⌝ ∗
     meta l nroot γ ∗
-    inv nroot (inv_inner l γ).
+    inv' l γ Ψ.
   #[local] Instance : CustomIpatFormat "inv" :=
     "(
       %l &
       %γ &
-      -> &
       -> &
       -> &
       #Hmeta &
@@ -232,15 +233,23 @@ Section rcfd_G.
       #Hlstate_lb
     )".
 
-  #[global] Instance rcfd_inv_timeless t q :
-    Timeless (rcfd_token t q).
+  #[global] Instance rcfd_inv_contractive t fd n :
+    Proper (
+      (pointwise_relation _ (dist_later n)) ==>
+      (≡{n}≡)
+    ) (rcfd_inv t fd).
   Proof.
-    apply _.
+    rewrite /rcfd_inv /inv' /inv_inner /inv_inner_open /inv_inner_closing_users.
+    solve_contractive.
   Qed.
-  #[global] Instance rcfd_inv_persistent t fd chars :
-    Persistent (rcfd_inv t fd chars).
+  #[global] Instance rcfd_inv_proper t fd :
+    Proper (
+      (pointwise_relation _ (≡)) ==>
+      (≡)
+    ) (rcfd_inv t fd).
   Proof.
-    apply _.
+    rewrite /rcfd_inv /inv' /inv_inner /inv_inner_open /inv_inner_closing_users.
+    solve_proper.
   Qed.
 
   #[global] Instance rcfd_token_timeless t q :
@@ -248,9 +257,13 @@ Section rcfd_G.
   Proof.
     apply _.
   Qed.
-
   #[global] Instance rcfd_closing_timeless t :
     Timeless (rcfd_closing t).
+  Proof.
+    apply _.
+  Qed.
+  #[global] Instance rcfd_inv_persistent t fd Ψ :
+    Persistent (rcfd_inv t fd Ψ).
   Proof.
     apply _.
   Qed.
@@ -348,27 +361,26 @@ Section rcfd_G.
     apply auth_mono_update'.
   Qed.
 
-  Lemma rcfd_make_spec fd chars :
+  Lemma rcfd_make_spec Ψ fd :
     {{{
-      unix_fd_model fd (DfracOwn 1) chars
+      Ψ 1%Qp
     }}}
       rcfd_make fd
     {{{ t,
       RET t;
-      rcfd_inv t fd chars
+      rcfd_inv t fd Ψ
     }}}.
   Proof.
-    iIntros "%Φ Hmodel HΦ".
+    iIntros "%Φ HΨ HΦ".
 
     wp_rec.
     wp_block_generative open.
-    wp_block l as "Hmeta" "(Hops & Hfd & _)".
+    wp_block l as "Hmeta" "(Hl_ops & Hl_fd & _)".
 
     iMod tokens_alloc as "(%γ_tokens & Htokens_auth)".
     iMod lstate_alloc as "(%γ_lstate & Hlstate_auth)".
     pose γ := {|
       metadata_fd := fd ;
-      metadata_chars := chars ;
       metadata_open := open ;
       metadata_tokens := γ_tokens ;
       metadata_lstate := γ_lstate ;
@@ -376,17 +388,18 @@ Section rcfd_G.
     iMod (meta_set γ with "Hmeta") as "#Hmeta"; first done.
 
     iApply "HΦ".
-    iExists l, γ. iSteps. iExists Open. iSteps. iExists ∅. iSteps.
+    iExists l, γ. iSteps.
+    iExists Open. iSteps.
+    iExists ∅. iSteps.
   Qed.
 
-  #[local] Lemma rcfd_put_spec' l γ :
+  #[local] Lemma rcfd_put_spec_aux l γ Ψ `{!Fractional Ψ} :
     {{{
-      inv nroot (inv_inner l γ) ∗
-      ( ( ∃ q,
-          tokens_frag γ q ∗
-          unix_fd_model γ.(metadata_fd) (DfracOwn q) γ.(metadata_chars)
-        )
-      ∨ lstate_lb γ LClosingNoUsers
+      inv' l γ Ψ ∗
+      ( lstate_lb γ LClosingNoUsers
+      ∨ ∃ q,
+        tokens_frag γ q ∗
+        Ψ q
       )
     }}}
       rcfd_put #l
@@ -403,20 +416,25 @@ Section rcfd_G.
     iInv "Hinv" as "(:inv_inner =1)".
     wp_faa.
     iSplitR "HΦ".
-    { iDestruct "H" as "[(%q & Htokens_frag & Hmodel) | #Hlstate_lb]".
+    { iDestruct "H" as "[#Hlstate_lb | (%q & Htokens_frag & HΨ)]".
+      - iDestruct (lstate_valid_closing_no_users with "Hlstate_auth Hlstate_lb") as %->.
+        iDestruct "Hlstate" as "(:inv_inner_closing_no_users =1)".
+        iExists (Closing _). iStep 4. done.
       - destruct lstate1.
-        + iDestruct "Hlstate" as "(:inv_inner_open =1)".
+        + iDestruct "Hlstate" as "(:inv_inner_open =1 !=)".
           iDestruct (tokens_elem_of with "Htokens_auth Htokens_frag") as %Hq.
           iExists Open. iStep 3. iExists (q + q1)%Qp, (qs1 ∖ {[+q+]}).
-          iSplitR; [iSplitR; iPureIntro | iSplitR; [| iSplitR "Hmodel Hmodel_"]].
+          iSplitR; [iSplitR; iPureIntro | iSplitR; [| iSplitR "HΨ HΨ_"]].
           * assert (qs1 ≠ ∅) as Hqs1_size%gmultiset_size_non_empty_iff by multiset_solver.
             rewrite gmultiset_size_difference; first multiset_solver.
             rewrite gmultiset_size_singleton. lia.
           * rewrite (gmultiset_disj_union_difference' q qs1) // gmultiset_set_fold_disj_union gmultiset_set_fold_singleton // in Hqs1.
           * iSteps.
-          * iMod (tokens_update_dealloc with "Htokens_auth Htokens_frag") as "$". iSteps.
-          * iCombine "Hmodel Hmodel_" as "$". iSteps.
-        + iDestruct "Hlstate" as "(:inv_inner_closing_users =1)".
+          * iMod (tokens_update_dealloc with "Htokens_auth Htokens_frag") as "$".
+            iSteps.
+          * iDestruct (fractional with "[$HΨ $HΨ_]") as "$".
+            iSteps.
+        + iDestruct "Hlstate" as "(:inv_inner_closing_users =1 !=)".
           iDestruct (tokens_elem_of with "Htokens_auth Htokens_frag") as %Hq.
           destruct (decide (size qs1 = 1)) as [Hqs_size' | Hqs_size'].
           * apply gmultiset_size_1_elem_of in Hqs_size' as (q_ & ->%leibniz_equiv). rewrite gmultiset_set_fold_singleton in Hqs1.
@@ -424,25 +442,23 @@ Section rcfd_G.
             iMod (tokens_update_dealloc with "Htokens_auth Htokens_frag") as "Htokens_auth".
             rewrite gmultiset_difference_diag.
             iMod (lstate_update LClosingNoUsers with "Hlstate_auth") as "Hlstate_auth"; first done.
-            iCombine "Hmodel Hmodel_" as "Hmodel". rewrite Hqs1. iDestruct ("Hfn1" with "Hmodel") as "Hfn1".
-            iExists (Closing _). iStep 4. done.
+            iDestruct (fractional with "[$HΨ $HΨ_]") as "HΨ". rewrite Hqs1.
+            iFrameSteps 2.
           * iMod (tokens_update_dealloc with "Htokens_auth Htokens_frag") as "Htokens_auth".
-            iCombine "Hmodel Hmodel_" as "Hmodel".
-            iExists (Closing _). iStep 3. iExists (q + q1)%Qp, (qs1 ∖ {[+q+]}). iSteps; iPureIntro.
+            iDestruct (fractional with "[$HΨ $HΨ_]") as "HΨ".
+            iFrameSteps 2; iPureIntro.
             -- rewrite gmultiset_size_difference; first multiset_solver.
                rewrite gmultiset_size_singleton. lia.
             -- rewrite gmultiset_size_difference; first multiset_solver.
                rewrite gmultiset_size_singleton. lia.
             -- rewrite (gmultiset_disj_union_difference' q qs1) // gmultiset_set_fold_disj_union gmultiset_set_fold_singleton // in Hqs1.
         + iDestruct "Hlstate" as "(:inv_inner_closing_no_users =1)".
-          iExists (Closing _). iStep 4. done.
-      - iDestruct (lstate_valid_closing_no_users with "Hlstate_auth Hlstate_lb") as %->.
-        iDestruct "Hlstate" as "(:inv_inner_closing_no_users =1)".
-        iExists (Closing _). iStep 4. done.
+          iFrameSteps 2.
     }
-    iModIntro. clear.
+    iIntros "!> {%}".
 
-    wp_pures. destruct (decide (ops1 = 1)) as [-> | Hops]; wp_pures; last iSteps.
+    wp_pures.
+    destruct (decide (ops1 = 1)) as [-> | Hops]; wp_pures; last iSteps.
 
     wp_bind (_.{state})%E.
     iInv "Hinv" as "(:inv_inner =2)".
@@ -450,21 +466,26 @@ Section rcfd_G.
     destruct (decide (lstate2 = LOpen)) as [-> | Hlstate2].
 
     - iDestruct "Hlstate" as "(:inv_inner_open =2)".
-      iSplitR "HΦ". { iExists Open. iSteps. }
+      iSplitR "HΦ". { iFrameSteps 2. }
       iSteps.
 
-    - iAssert (∃ fn2, ⌜state2 = Closing fn2⌝ ∗ lstate_lb γ LClosingUsers)%I as "(%fn2 & -> & #Hlstate_lb)".
+    - iAssert (
+        ∃ fn2,
+        ⌜state2 = Closing fn2⌝ ∗
+        lstate_lb γ LClosingUsers
+      )%I as "(%fn2 & -> & #Hlstate_lb)".
       { destruct lstate2; first done.
         - iDestruct "Hlstate" as "(:inv_inner_closing_users =2)".
           iDestruct (lstate_lb_get with "Hlstate_auth") as "$".
           iSteps.
         - iDestruct "Hlstate" as "(:inv_inner_closing_no_users =2)".
           iDestruct (lstate_lb_get with "Hlstate_auth") as "Hlstate_lb".
-          iDestruct (lstate_lb_mono LClosingUsers with "Hlstate_lb") as "Hlstate_lb"; first done.
+          iDestruct (lstate_lb_mono LClosingUsers with "Hlstate_lb") as "$"; first done.
           iSteps.
       }
-      iSplitR "HΦ". { iExists (Closing _). iSteps. }
-      iModIntro. clear.
+
+      iSplitR "HΦ". { iFrameSteps 2. }
+      iIntros "!> {%}".
 
       wp_pures.
 
@@ -474,13 +495,13 @@ Section rcfd_G.
       iDestruct (lstate_valid_closing_users with "Hlstate_auth Hlstate_lb") as %[-> | ->].
 
       + iDestruct "Hlstate" as "(:inv_inner_closing_users =3)".
-        iSplitR "HΦ". { iExists (Closing _). iSteps. }
+        iSplitR "HΦ". { iFrameSteps 2. }
         iSteps.
 
       + iDestruct "Hlstate" as "(:inv_inner_closing_no_users =3)".
         iClear "Hlstate_lb". iDestruct (lstate_lb_get with "Hlstate_auth") as "#Hlstate_lb".
-        iSplitR "HΦ". { iExists (Closing _). iStep 4. done. }
-        iModIntro. clear.
+        iSplitR "HΦ". { iFrameSteps 2. }
+        iIntros "!> {%}".
 
         wp_pures. case_bool_decide as Hops3; wp_pures; last iSteps.
 
@@ -491,14 +512,15 @@ Section rcfd_G.
         destruct Hcas as (_ & _ & [= <-]).
         iDestruct (lstate_valid_closing_no_users with "Hlstate_auth Hlstate_lb") as %->.
         iDestruct "Hlstate" as "(:inv_inner_closing_no_users =4 eq)". injection Heq as <-.
-        iSplitR "Hfn4 HΦ". { iExists (Closing _). iSteps. }
+        iSplitR "Hfn4 HΦ".
+        { iExists (Closing _). iFrameSteps. }
         iSteps.
   Qed.
-  #[local] Lemma rcfd_put_spec t fd chars q :
+  #[local] Lemma rcfd_put_spec t fd Ψ `{!Fractional Ψ} q :
     {{{
-      rcfd_inv t fd chars ∗
+      rcfd_inv t fd Ψ ∗
       rcfd_token t q ∗
-      unix_fd_model fd (DfracOwn q) chars
+      Ψ q
     }}}
       rcfd_put t
     {{{
@@ -506,15 +528,14 @@ Section rcfd_G.
       True
     }}}.
   Proof.
-    iIntros "%Φ ((:inv) & (:token) & Hmodel) HΦ". injection Heq as <-.
+    iIntros "%Φ ((:inv) & (:token) & HΨ) HΦ". injection Heq as <-.
     iDestruct (meta_agree with "Hmeta Hmeta_") as %<-. iClear "Hmeta_".
-    iApply (rcfd_put_spec' with "[$Hinv Htokens_frag Hmodel] HΦ").
-    iSteps.
+    iApply (rcfd_put_spec_aux with "[$Hinv Htokens_frag HΨ] HΦ"); first iSteps.
   Qed.
 
-  #[local] Lemma rcfd_get_spec t fd chars :
+  #[local] Lemma rcfd_get_spec t fd Ψ `{HΨ : !Fractional Ψ} :
     {{{
-      rcfd_inv t fd chars
+      rcfd_inv t fd Ψ
     }}}
       rcfd_get t
     {{{ o,
@@ -526,7 +547,7 @@ Section rcfd_G.
           ∃ q,
           ⌜fd_ = fd⌝ ∗
           rcfd_token t q ∗
-          unix_fd_model fd (DfracOwn q) chars
+          Ψ q
       end
     }}}.
   Proof.
@@ -537,37 +558,37 @@ Section rcfd_G.
     wp_bind (FAA _ _).
     iInv "Hinv" as "(:inv_inner =1)".
     wp_faa.
+
     iAssert (|==>
-      inv_inner l γ ∗
-      ( ( ∃ q,
-          tokens_frag γ q ∗
-          unix_fd_model γ.(metadata_fd) (DfracOwn q) γ.(metadata_chars)
-        )
-      ∨ lstate_lb γ LClosingNoUsers
+      inv_inner l γ Ψ ∗
+      ( lstate_lb γ LClosingNoUsers
+      ∨ ∃ q,
+        tokens_frag γ q ∗
+        Ψ q
       )
     )%I with "[- HΦ]" as ">($ & H)".
     { destruct lstate1.
       - iDestruct "Hlstate" as "(:inv_inner_open)".
         iMod (tokens_update_alloc (q / 2) with "Htokens_auth") as "(Htokens_auth & Htokens_frag)".
-        iDestruct "Hmodel_" as "(Hmodel1 & Hmodel2)".
-        iSplitR "Htokens_frag Hmodel2"; last iSteps.
-        iExists Open. iStep 3. iExists (q / 2)%Qp, ({[+q / 2+]} ⊎ qs)%Qp. iSteps; iPureIntro.
+        iDestruct (fractional_half with "HΨ") as "(HΨ1 & HΨ2)"; first done.
+        iSplitR "Htokens_frag HΨ2"; last iSteps.
+        iFrameSteps 2; iPureIntro.
         + rewrite gmultiset_size_disj_union gmultiset_size_singleton. lia.
         + rewrite gmultiset_set_fold_disj_union gmultiset_set_fold_singleton Qp.div_2 //.
       - iDestruct "Hlstate" as "(:inv_inner_closing_users)".
         iMod (tokens_update_alloc (q / 2) with "Htokens_auth") as "(Htokens_auth & Htokens_frag)".
-        iDestruct "Hmodel_" as "(Hmodel1 & Hmodel2)".
-        iSplitR "Htokens_frag Hmodel2"; last iSteps.
-        iExists (Closing _). iStep 3. iExists (q / 2)%Qp, ({[+q / 2+]} ⊎ qs)%Qp. iSteps; iPureIntro.
+        iDestruct (fractional_half with "HΨ") as "(HΨ1 & HΨ2)"; first done.
+        iSplitR "Htokens_frag HΨ2"; last iSteps.
+        iFrameSteps 2; iPureIntro.
         + rewrite gmultiset_size_disj_union gmultiset_size_singleton. lia.
         + rewrite gmultiset_size_disj_union. lia.
         + rewrite gmultiset_set_fold_disj_union gmultiset_set_fold_singleton Qp.div_2 //.
       - iDestruct "Hlstate" as "(:inv_inner_closing_no_users)".
         iDestruct (lstate_lb_get with "Hlstate_auth") as "#Hlstate_lb".
-        iSplitL; last iSteps.
-        iExists (Closing _). iSteps.
+        iFrameSteps 2.
     }
-    iModIntro. wp_pures. clear.
+
+    iModIntro. wp_pures. clear- HΨ.
 
     wp_bind (_.{state})%E.
     iInv "Hinv" as "(:inv_inner =2)".
@@ -575,30 +596,38 @@ Section rcfd_G.
     destruct (decide (lstate2 = LOpen)) as [-> | Hlstate2].
 
     - iDestruct "Hlstate" as "(:inv_inner_open)".
-      iDestruct "H" as "[(%q' & Htokens_frag & Hmodel) | Hlstate_lb]"; last first.
+      iDestruct "H" as "[#Hlstate_lb | (%q' & Htokens_frag & HΨ_)]".
       { iDestruct (lstate_valid_closing_no_users with "Hlstate_auth Hlstate_lb") as %?. done. }
-      iSplitR "Htokens_frag Hmodel HΦ". { iExists Open. iSteps. }
-      iModIntro. clear.
+      iSplitR "Htokens_frag HΨ_ HΦ". { iFrameSteps 2. }
+      iIntros "!> {%}".
 
       wp_pures.
       iApply ("HΦ" $! (Some _)). iSteps.
 
-    - iAssert ⌜∃ fn2, state2 = Closing fn2⌝%I as %(fn2 & ->).
+    - iAssert (
+        ∃ fn2,
+        ⌜state2 = Closing fn2⌝
+      )%I as %(fn2 & ->).
       { destruct lstate2; iDecompose "Hlstate"; iSteps. }
-      iSplitR "H HΦ". { iExists (Closing fn2). iSteps. }
-      iModIntro. clear.
 
-      wp_smart_apply (rcfd_put_spec' with "[$]") as "_".
-      iSteps. iApply ("HΦ" $! None). iSteps.
+      iSplitR "H HΦ". { iFrameSteps 2. }
+      iModIntro. clear- HΨ.
+
+      wp_smart_apply (rcfd_put_spec_aux with "[$]") as "_".
+      wp_pures.
+      iApply ("HΦ" $! None). iSteps.
   Qed.
 
-  #[local] Lemma rcfd_close_spec' closing t fd chars :
+  #[local] Lemma rcfd_close_spec_aux closing t fd Ψ :
     {{{
-      rcfd_inv t fd chars ∗
+      rcfd_inv t fd Ψ ∗
       if closing then
         rcfd_closing t
       else
-        True
+        ( Ψ 1%Qp -∗
+            ∃ chars,
+            unix_fd_model fd (DfracOwn 1) chars
+        )
     }}}
       rcfd_close t
     {{{ b,
@@ -619,13 +648,14 @@ Section rcfd_G.
     destruct (decide (lstate1 = LOpen)) as [-> | Hlstate1].
 
     - iDestruct "Hlstate" as "(:inv_inner_open =1)".
-      destruct closing; last iClear "Hclosing".
+      destruct closing.
       { iDestruct "Hclosing" as "(:closing)". injection Heq as <-.
         iDestruct (meta_agree with "Hmeta Hmeta_") as %<-. iClear "Hmeta_".
         iDestruct (lstate_valid_closing_users with "Hlstate_auth Hlstate_lb") as %[[=] | [=]].
       }
-      iSplitR "HΦ". { iExists Open. iSteps. }
-      iModIntro. clear.
+
+      iSplitR "Hclosing HΦ". { iFrameSteps 2. }
+      iIntros "!> {%}".
 
       wp_pures.
 
@@ -633,7 +663,11 @@ Section rcfd_G.
       iInv "Hinv" as "(:inv_inner =2)".
       wp_cas as Hcas.
 
-      + iAssert (⌜∃ fn2, state2 = Closing fn2⌝ ∗ lstate_lb γ LClosingUsers)%I as "((%fn2 & ->) & #Hlstate_lb)".
+      + iAssert (
+          ∃ fn2,
+          ⌜state2 = Closing fn2⌝ ∗
+          lstate_lb γ LClosingUsers
+        )%I as "(%fn2 & -> & #Hlstate_lb)".
         { destruct lstate2; iDecompose "Hlstate".
           - zoo_simpl. naive_solver.
           - iDestruct (lstate_lb_get with "Hlstate_auth") as "$".
@@ -642,7 +676,8 @@ Section rcfd_G.
             iDestruct (lstate_lb_mono with "Hlstate_lb") as "$"; first done.
             iSteps.
         }
-        iSplitR "HΦ". { iExists (Closing _). iSteps. }
+
+        iSplitR "HΦ". { iFrameSteps 2. }
         iSteps.
 
       + destruct state2; last zoo_simpl.
@@ -651,32 +686,34 @@ Section rcfd_G.
         iDestruct "Hlstate" as "(:inv_inner_open =2 eq)".
         iMod (lstate_update LClosingUsers with "Hlstate_auth") as "Hlstate_auth"; first done.
         iDestruct (lstate_lb_get with "Hlstate_auth") as "#Hlstate_lb".
+
         iSplitR "HΦ".
         { destruct (decide (size qs2 = 0)) as [Hqs_size | Hqs_size].
           - apply gmultiset_size_empty_iff in Hqs_size as ->.
             rewrite gmultiset_set_fold_empty in Hqs2. rewrite {}Hqs2.
             iMod (lstate_update LClosingNoUsers with "Hlstate_auth") as "Hlstate_auth"; first done.
-            iExists (Closing _). iSteps.
-            wp_apply (unix_close_spec with "[$]").
-            iSteps.
-          - iExists (Closing _). iSteps.
-            wp_apply (unix_close_spec with "[$]").
+            iDestruct ("Hclosing" with "HΨ") as "(%chars & Hfd)".
+            iExists (Closing _). iFrameSteps.
+          - iExists (Closing _). iFrame. iStep 3 as "HΨ".
+            iDestruct ("Hclosing" with "HΨ") as "(%chars & Hfd)".
             iSteps.
         }
-        iModIntro. clear.
+        iIntros "!> {%}".
 
         wp_pures.
 
         wp_bind (_.{ops})%E.
         iInv "Hinv" as "(:inv_inner =3)".
         wp_load.
+
         destruct (decide (ops3 = 0)) as [-> | Hops3]; last iSteps.
+
         iDestruct (lstate_valid_closing_users with "Hlstate_auth Hlstate_lb") as %[-> | ->].
         { iDestruct "Hlstate" as "(:inv_inner_closing_users =3 eq_ops)". lia. }
         iDestruct "Hlstate" as "(:inv_inner_closing_no_users =3)".
         iRename "Hlstate_lb" into "Hlstate_lb'". iDestruct (lstate_lb_get with "Hlstate_auth") as "#Hlstate_lb".
-        iSplitR "HΦ". { iExists (Closing _). iStep 4. done. }
-        iModIntro. clear.
+        iSplitR "HΦ". { iFrameSteps 2. }
+        iIntros "!> {%}".
 
         wp_pures.
 
@@ -687,13 +724,18 @@ Section rcfd_G.
         iDestruct (lstate_valid_closing_no_users with "Hlstate_auth Hlstate_lb") as %->.
         iDestruct "Hlstate" as "(:inv_inner_closing_no_users =4)".
         destruct Hcas as (_ & _ & [= ->]).
-        iSplitR "Hfn4 HΦ". { iExists (Closing _). iSteps. }
-        iModIntro. clear.
+        iSplitR "Hfn4 HΦ".
+        { iExists (Closing _). iFrameSteps. }
+        iIntros "!> {%}".
 
         wp_smart_apply (wp_wand with "Hfn4").
         iSteps.
 
-    - iAssert (⌜∃ fn1, state1 = Closing fn1⌝ ∗ lstate_lb γ LClosingUsers)%I as "((%fn1 & ->) & #Hlstate_lb)".
+    - iAssert (
+        ∃ fn1,
+        ⌜state1 = Closing fn1⌝ ∗
+        lstate_lb γ LClosingUsers
+      )%I as "(%fn1 & -> & #Hlstate_lb)".
       { destruct lstate1; iDecompose "Hlstate".
         - iDestruct (lstate_lb_get with "Hlstate_auth") as "$".
           iSteps.
@@ -701,12 +743,20 @@ Section rcfd_G.
           iDestruct (lstate_lb_mono with "Hlstate_lb") as "$"; first done.
           iSteps.
       }
-      iSplitR "HΦ". { iExists (Closing _). iSteps. }
-      iSteps. destruct closing; iSteps.
+
+      iSplitR "HΦ". { iFrameSteps 2. }
+      iIntros "!> {%}".
+
+      wp_pures.
+      destruct closing; iSteps.
   Qed.
-  Lemma rcfd_close_spec t fd chars :
+  Lemma rcfd_close_spec t fd Ψ :
     {{{
-      rcfd_inv t fd chars
+      rcfd_inv t fd Ψ ∗
+      ( Ψ 1%Qp -∗
+          ∃ chars,
+          unix_fd_model fd (DfracOwn 1) chars
+      )
     }}}
       rcfd_close t
     {{{ b,
@@ -714,13 +764,12 @@ Section rcfd_G.
       rcfd_closing t
     }}}.
   Proof.
-    iIntros "%Φ #Hinv HΦ".
-    wp_apply (rcfd_close_spec' false with "[$Hinv]").
-    iSteps.
+    iIntros "%Φ (#Hinv & H) HΦ".
+    wp_apply (rcfd_close_spec_aux false with "[$] HΦ").
   Qed.
-  Lemma rcfd_close_spec_closing t fd chars :
+  Lemma rcfd_close_spec_closing t fd Ψ :
     {{{
-      rcfd_inv t fd chars ∗
+      rcfd_inv t fd Ψ ∗
       rcfd_closing t
     }}}
       rcfd_close t
@@ -730,13 +779,13 @@ Section rcfd_G.
     }}}.
   Proof.
     iIntros "%Φ (#Hinv & #Hclosing) HΦ".
-    wp_apply (rcfd_close_spec' true with "[$Hinv $Hclosing]").
+    wp_apply (rcfd_close_spec_aux true with "[$]").
     iSteps.
   Qed.
 
-  #[local] Lemma rcfd_remove_spec' closing t fd chars :
+  #[local] Lemma rcfd_remove_spec_aux closing t fd Ψ :
     {{{
-      rcfd_inv t fd chars ∗
+      rcfd_inv t fd Ψ ∗
       if closing then
         rcfd_closing t
       else
@@ -754,7 +803,7 @@ Section rcfd_G.
             True
         | Some fd_ =>
             ⌜fd_ = fd⌝ ∗
-            unix_fd_model fd (DfracOwn 1) chars
+            Ψ 1%Qp
         end
     }}}.
   Proof.
@@ -773,17 +822,22 @@ Section rcfd_G.
         iDestruct (meta_agree with "Hmeta Hmeta_") as %<-. iClear "Hmeta_".
         iDestruct (lstate_valid_closing_users with "Hlstate_auth Hlstate_lb") as %[[=] | [=]].
       }
-      iSplitR "HΦ". { iExists Open. iSteps. }
-      iModIntro. clear.
 
-      wp_smart_apply (spsc_waiter_create_spec (unix_fd_model γ.(metadata_fd) (DfracOwn 1) γ.(metadata_chars)) with "[//]") as "%chan (#Hchan_inv & Hchan_producer & Hchan_consumer)".
+      iSplitR "HΦ". { iFrameSteps 2. }
+      iIntros "!> {%}".
+
+      wp_smart_apply (spsc_waiter_create_spec (Ψ 1%Qp) with "[//]") as "%waiter (#Hwaiter_inv & Hwaiter_producer & Hwaiter_consumer)".
       wp_pures.
 
       wp_bind (CAS _ _ _).
       iInv "Hinv" as "(:inv_inner =2)".
       wp_cas as Hcas.
 
-      + iAssert (⌜∃ fn2, state2 = Closing fn2⌝ ∗ lstate_lb γ LClosingUsers)%I as "((%fn2 & ->) & #Hlstate_lb)".
+      + iAssert (
+          ∃ fn2,
+          ⌜state2 = Closing fn2⌝ ∗
+          lstate_lb γ LClosingUsers
+        )%I as "(%fn2 & -> & #Hlstate_lb)".
         { destruct lstate2; iDecompose "Hlstate".
           - zoo_simpl. naive_solver.
           - iDestruct (lstate_lb_get with "Hlstate_auth") as "$".
@@ -792,8 +846,12 @@ Section rcfd_G.
             iDestruct (lstate_lb_mono with "Hlstate_lb") as "$"; first done.
             iSteps.
         }
-        iSplitR "HΦ". { iExists (Closing _). iSteps. }
-        iSteps. iApply ("HΦ" $! None). iSteps.
+
+        iSplitR "HΦ". { iFrameSteps 2. }
+        iIntros "!> {%}".
+
+        wp_pures.
+        iApply ("HΦ" $! None). iSteps.
 
       + destruct state2; last zoo_simpl.
         destruct (decide (lstate2 = LOpen)) as [-> | Hlstate2]; last first.
@@ -801,24 +859,29 @@ Section rcfd_G.
         iDestruct "Hlstate" as "(:inv_inner_open =2 eq)".
         iMod (lstate_update LClosingUsers with "Hlstate_auth") as "Hlstate_auth"; first done.
         iDestruct (lstate_lb_get with "Hlstate_auth") as "#Hlstate_lb".
-        iSplitR "Hchan_consumer HΦ".
+        iSplitR "Hwaiter_consumer HΦ".
         { destruct (decide (size qs2 = 0)) as [Hqs_size | Hqs_size].
           - apply gmultiset_size_empty_iff in Hqs_size as ->.
             rewrite gmultiset_set_fold_empty in Hqs2. rewrite {}Hqs2.
             iMod (lstate_update LClosingNoUsers with "Hlstate_auth") as "Hlstate_auth"; first done.
-            iExists (Closing _). iStep 8.
-            wp_apply (spsc_waiter_notify_spec with "[$Hchan_inv $Hchan_producer $Hmodel_]").
+            iExists (Closing _). iFrameStep 8.
+            wp_apply (spsc_waiter_notify_spec with "[$Hwaiter_inv $Hwaiter_producer $HΨ]").
             iSteps.
-          - iExists (Closing _). iSteps as "Hmodel".
-            wp_apply (spsc_waiter_notify_spec with "[$Hchan_inv $Hchan_producer $Hmodel]").
+          - iExists (Closing _). iFrame. iSteps as "HΨ".
+            wp_apply (spsc_waiter_notify_spec with "[$Hwaiter_inv $Hwaiter_producer $HΨ]").
             iSteps.
         }
-        iModIntro. clear.
+        iIntros "!> {%}".
 
-        wp_smart_apply (spsc_waiter_wait_spec with "[$Hchan_inv $Hchan_consumer]") as "Hmodel".
-        iSteps. iApply ("HΦ" $! (Some _)). iSteps.
+        wp_smart_apply (spsc_waiter_wait_spec with "[$Hwaiter_inv $Hwaiter_consumer]") as "HΨ".
+        wp_pures.
+        iApply ("HΦ" $! (Some _)). iSteps.
 
-    - iAssert (⌜∃ fn1, state1 = Closing fn1⌝ ∗ lstate_lb γ LClosingUsers)%I as "((%fn1 & ->) & #Hlstate_lb)".
+    - iAssert (
+        ∃ fn1,
+        ⌜state1 = Closing fn1⌝ ∗
+        lstate_lb γ LClosingUsers
+      )%I as "(%fn1 & -> & #Hlstate_lb)".
       { destruct lstate1; iDecompose "Hlstate".
         - iDestruct (lstate_lb_get with "Hlstate_auth") as "$".
           iSteps.
@@ -826,12 +889,16 @@ Section rcfd_G.
           iDestruct (lstate_lb_mono with "Hlstate_lb") as "$"; first done.
           iSteps.
       }
-      iSplitR "HΦ". { iExists (Closing _). iSteps. }
-      iSteps. iApply ("HΦ" $! None). destruct closing; iSteps.
+
+      iSplitR "HΦ". { iFrameSteps 2. }
+      iIntros "!> {%}".
+
+      wp_pures.
+      iApply ("HΦ" $! None). destruct closing; iSteps.
   Qed.
-  Lemma rcfd_remove_spec t fd chars :
+  Lemma rcfd_remove_spec t fd Ψ :
     {{{
-      rcfd_inv t fd chars
+      rcfd_inv t fd Ψ
     }}}
       rcfd_remove t
     {{{ o,
@@ -842,17 +909,16 @@ Section rcfd_G.
           True
       | Some fd_ =>
           ⌜fd_ = fd⌝ ∗
-          unix_fd_model fd (DfracOwn 1) chars
+          Ψ 1%Qp
       end
     }}}.
   Proof.
     iIntros "%Φ #Hinv HΦ".
-    wp_apply (rcfd_remove_spec' false with "[$Hinv]").
-    iSteps.
+    wp_apply (rcfd_remove_spec_aux false with "[$Hinv] HΦ").
   Qed.
-  Lemma rcfd_remove_spec_closing closing t fd chars :
+  Lemma rcfd_remove_spec_closing closing t fd Ψ :
     {{{
-      rcfd_inv t fd chars ∗
+      rcfd_inv t fd Ψ ∗
       rcfd_closing t
     }}}
       rcfd_remove t
@@ -862,42 +928,42 @@ Section rcfd_G.
     }}}.
   Proof.
     iIntros "%Φ (#Hinv & #Hclosing) HΦ".
-    wp_apply (rcfd_remove_spec' true with "[$Hinv $Hclosing]").
+    wp_apply (rcfd_remove_spec_aux true with "[$Hinv $Hclosing]").
     iSteps.
   Qed.
 
-  Lemma rcfd_use_spec Ψ t fd chars (closed open : val) :
+  Lemma rcfd_use_spec Χ t fd Ψ `{!Fractional Ψ} (closed open : val) :
     {{{
-      rcfd_inv t fd chars ∗
-      WP closed () {{ Ψ false }} ∗
+      rcfd_inv t fd Ψ ∗
+      WP closed () {{ Χ false }} ∗
       ( ∀ q,
         rcfd_token t q -∗
-        unix_fd_model fd (DfracOwn q) chars -∗
+        Ψ q -∗
         WP open fd {{ res,
           rcfd_token t q ∗
-          unix_fd_model fd (DfracOwn q) chars ∗
-          Ψ true res
+          Ψ q ∗
+          Χ true res
         }}
       )
     }}}
       rcfd_use t closed open
     {{{ b res,
       RET res;
-      Ψ b res
+      Χ b res
     }}}.
   Proof.
     iIntros "%Φ (#Hinv & Hclosed & Hopen) HΦ".
     wp_rec.
     wp_smart_apply (rcfd_get_spec with "Hinv") as ([]) ""; last iSteps.
-    iIntros "(%q & -> & Htoken & Hmodel)".
-    wp_smart_apply (wp_wand with "(Hopen Htoken Hmodel)") as "%res (Htoken & Hmodel & HΨ)".
-    wp_smart_apply (rcfd_put_spec with "[$Hinv $Htoken $Hmodel]").
+    iIntros "(%q & -> & Htoken & HΨ)".
+    wp_smart_apply (wp_wand with "(Hopen Htoken HΨ)") as "%res (Htoken & HΨ & HΧ)".
+    wp_smart_apply (rcfd_put_spec with "[$Hinv $Htoken $HΨ]").
     iSteps.
   Qed.
 
-  #[local] Lemma rcfd_is_open_spec' closing t fd chars :
+  #[local] Lemma rcfd_is_open_spec_aux closing t fd Ψ :
     {{{
-      rcfd_inv t fd chars ∗
+      rcfd_inv t fd Ψ ∗
       if closing then
         rcfd_closing t
       else
@@ -921,20 +987,25 @@ Section rcfd_G.
     wp_bind (_.{state})%E.
     iInv "Hinv" as "(:inv_inner)".
     wp_load.
-    destruct closing; last iClear "Hclosing".
+    destruct closing.
 
     - iDestruct "Hclosing" as "(:closing)". injection Heq as <-.
       iDestruct (meta_agree with "Hmeta Hmeta_") as %<-. iClear "Hmeta_".
-      iAssert ⌜∃ fn, state = Closing fn⌝%I as %(fn & ->).
+
+      iAssert (
+        ∃ fn,
+        ⌜state = Closing fn⌝
+      )%I as "(%fn & ->)".
       { iDestruct (lstate_valid_closing_users with "Hlstate_auth Hlstate_lb") as %[-> | ->].
         all: iDecompose "Hlstate"; iSteps.
       }
-      iSplitR "HΦ". { iExists (Closing _). iSteps. }
+
+      iSplitR "HΦ". { iFrameSteps 2. }
       iSteps.
 
     - destruct state.
 
-      + iSplitR "HΦ". { iExists Open. iSteps. }
+      + iSplitR "HΦ". { iFrameSteps 2. }
         iSteps.
 
       + iAssert (lstate_lb γ LClosingUsers) as "#Hlstate_lb".
@@ -943,12 +1014,13 @@ Section rcfd_G.
           - iDestruct (lstate_lb_get with "Hlstate_auth") as "Hlstate_lb".
             iApply (lstate_lb_mono with "Hlstate_lb"); first done.
         }
-        iSplitR "HΦ". { iExists (Closing _). iSteps. }
+
+        iSplitR "HΦ". { iFrameSteps 2. }
         iSteps.
   Qed.
-  Lemma rcfd_is_open_spec t fd chars :
+  Lemma rcfd_is_open_spec t fd Ψ :
     {{{
-      rcfd_inv t fd chars
+      rcfd_inv t fd Ψ
     }}}
       rcfd_is_open t
     {{{ b,
@@ -960,12 +1032,11 @@ Section rcfd_G.
     }}}.
   Proof.
     iIntros "%Φ #Hinv HΦ".
-    wp_apply (rcfd_is_open_spec' false with "[$Hinv]").
-    iSteps.
+    wp_apply (rcfd_is_open_spec_aux false with "[$Hinv] HΦ").
   Qed.
-  Lemma rcfd_is_open_spec_closing t fd chars :
+  Lemma rcfd_is_open_spec_closing t fd Ψ :
     {{{
-      rcfd_inv t fd chars ∗
+      rcfd_inv t fd Ψ ∗
       rcfd_closing t
     }}}
       rcfd_is_open t
@@ -975,13 +1046,13 @@ Section rcfd_G.
     }}}.
   Proof.
     iIntros "%Φ (#Hinv & #Hclosing) HΦ".
-    wp_apply (rcfd_is_open_spec' true with "[$Hinv $Hclosing]").
+    wp_apply (rcfd_is_open_spec_aux true with "[$Hinv $Hclosing]").
     iSteps.
   Qed.
 
-  #[local] Lemma rcfd_peek_spec' closing t fd chars :
+  #[local] Lemma rcfd_peek_spec_aux closing t fd Ψ :
     {{{
-      rcfd_inv t fd chars ∗
+      rcfd_inv t fd Ψ ∗
       if closing then
         rcfd_closing t
       else
@@ -1008,21 +1079,29 @@ Section rcfd_G.
     wp_bind (_.{state})%E.
     iInv "Hinv" as "(:inv_inner)".
     wp_load.
-    destruct closing; last iClear "Hclosing".
+    destruct closing.
 
     - iDestruct "Hclosing" as "(:closing)". injection Heq as <-.
       iDestruct (meta_agree with "Hmeta Hmeta_") as %<-. iClear "Hmeta_".
-      iAssert ⌜∃ fn, state = Closing fn⌝%I as %(fn & ->).
+
+      iAssert (
+        ∃ fn,
+        ⌜state = Closing fn⌝
+      )%I as "(%fn & ->)".
       { iDestruct (lstate_valid_closing_users with "Hlstate_auth Hlstate_lb") as %[-> | ->].
         all: iDecompose "Hlstate"; iSteps.
       }
-      iSplitR "HΦ". { iExists (Closing _). iSteps. }
-      iSteps. iApply ("HΦ" $! None). iSteps.
+
+      iSplitR "HΦ". { iFrameSteps 2. }
+      iIntros "!> {%}".
+
+      wp_pures.
+      iApply ("HΦ" $! None). iSteps.
 
     - destruct state.
 
-      + iSplitR "HΦ". { iExists Open. iSteps. }
-        iModIntro. clear.
+      + iSplitR "HΦ". { iFrameSteps 2. }
+        iIntros "!> {%}".
 
         wp_pures.
         iApply ("HΦ" $! (Some _)). iSteps.
@@ -1033,12 +1112,16 @@ Section rcfd_G.
           - iDestruct (lstate_lb_get with "Hlstate_auth") as "Hlstate_lb".
             iApply (lstate_lb_mono with "Hlstate_lb"); first done.
         }
-        iSplitR "HΦ". { iExists (Closing _). iSteps. }
-        iSteps. iApply ("HΦ" $! None). iSteps.
+
+        iSplitR "HΦ". { iFrameSteps 2. }
+        iIntros "!> {%}".
+
+        wp_pures.
+        iApply ("HΦ" $! None). iSteps.
   Qed.
-  Lemma rcfd_peek_spec t fd chars :
+  Lemma rcfd_peek_spec t fd Ψ :
     {{{
-      rcfd_inv t fd chars
+      rcfd_inv t fd Ψ
     }}}
       rcfd_peek t
     {{{ o,
@@ -1052,12 +1135,11 @@ Section rcfd_G.
     }}}.
   Proof.
     iIntros "%Φ #Hinv HΦ".
-    wp_apply (rcfd_peek_spec' false with "[$Hinv]").
-    iSteps.
+    wp_apply (rcfd_peek_spec_aux false with "[$Hinv] HΦ").
   Qed.
-  Lemma rcfd_peek_spec_closing t fd chars :
+  Lemma rcfd_peek_spec_closing t fd Ψ :
     {{{
-      rcfd_inv t fd chars ∗
+      rcfd_inv t fd Ψ ∗
       rcfd_closing t
     }}}
       rcfd_peek t
@@ -1067,7 +1149,7 @@ Section rcfd_G.
     }}}.
   Proof.
     iIntros "%Φ (#Hinv & #Hclosing) HΦ".
-    wp_apply (rcfd_peek_spec' true with "[$Hinv $Hclosing]").
+    wp_apply (rcfd_peek_spec_aux true with "[$Hinv $Hclosing]").
     iSteps.
   Qed.
 End rcfd_G.
